Added lemmas about pop

Pharoh/Queue.lean
@@ -4,15 +4,70 @@ structure Queue (α : Type u) : Type u where
   front : List α
   back : List α
 
-def push (x : α) (xs : Queue α) : Queue α := {
-  front := xs.front
-  back := x :: xs.back
-}
+namespace Queue
 
-def pop (x : α) (xs : Queue α) : Option (Queue α × α) :=
+instance : EmptyCollection (Queue α) := ⟨⟨[],[]⟩⟩
+
+@[simp]
+lemma empty_def : (∅ : Queue α) = ⟨[], []⟩ := rfl 
+
+def push (x : α) (xs : Queue α) : Queue α :=
+  {xs with back := x :: xs.back}
+
+@[simp]
+lemma push_def {x : α} : push x xs = {xs with back := x :: xs.back} := rfl 
+
+def pop (xs : Queue α) : Option (Queue α × α) :=
   match xs.front with
   | f :: fs => some ({back := xs.back, front := fs}, f)
   | [] => match xs.back.reverse with
           | b :: bs => some ({back := [], front := bs}, b)
           | nil => none
 
+@[simp]
+lemma pop_cons {f : α} {bs fs : List α} : 
+  pop {back := bs, front := f :: fs} = some (({back := bs, front := fs} : Queue α), f) := rfl
+
+@[simp]
+lemma pop_empty : pop (∅ : Queue α) = none := rfl
+
+theorem exists_head_of_reverse {bs : List α} (bsNotNil : bs ≠ []) : ∃ b' bs', bs.reverse = b' :: bs' := by
+  induction bs with
+  | nil => 
+    exfalso
+    apply bsNotNil rfl
+  | cons x xs ih =>
+    cases xs with
+    | nil => 
+      exists x; exists []; simp
+    | cons head tail =>
+      simp at *
+      cases ih with | intro b' ih =>
+      cases ih with | intro bs' ih =>
+      exists b'
+      exists (bs' ++ [x])
+      rw [ih]
+      simp
+
+theorem pop_flip_aux {bs : List α} :
+  pop {back := bs, front := []} = 
+          ( match bs.reverse with
+            | b :: bs => some ({back := [], front := bs}, b)
+            | nil => none
+          ) := by
+  rfl
+
+@[simp]
+lemma pop_flip {bs : List α} :
+  pop {back := bs, front := []} = pop {back := [], front := bs.reverse} := by
+    cases bs with
+    | nil => 
+      rw [List.reverse_nil, ← empty_def, pop_empty]
+    | cons b bs =>
+      have h := exists_head_of_reverse (List.noConfusion : (b :: bs) ≠ [])
+      cases h with | intro b' h =>
+      cases h with | intro bs' h =>
+      rw [pop_flip_aux, h]
+      simp
+
+end Queue
